Factor qualifier and store cores into prelude

ChoiceType/theories/Qualifier.v
@@ -1,106 +1,93 @@
 (** * ChoiceType.Qualifier
 
-    Type qualifiers are the source-level refinement predicates used by
-    choice types.  They remain shallow, locally-nameless predicates over a
-    vector of values.  Logic-level atoms live separately in
-    [ChoiceLogic.LogicQualifier]. *)
+    Type qualifiers are shallow Rocq predicates over stores.  Their syntax is
+    shared with logic qualifiers through [ChoicePrelude.Qualifier]; this file
+    specializes the generic qualifier result object to another store. *)
 
 From ChoiceType Require Export Prelude.
+From ChoicePrelude Require Import Qualifier.
 
 (** ** Syntax *)
 
-Inductive type_qualifier : Type :=
-  (** Standard shallow-embedding qualifier (like UnderType).
-      [vals] : the (possibly open) values the proposition mentions.
-      [prop] : a closed Rocq proposition over the evaluated constants. *)
-  | qual {n : nat} (vals : vec value n) (prop : vec constant n → Prop).
+Definition type_qualifier_of {V : Type} `{ValueSig V} : Type :=
+  qualifier (V := V) (A := gmap atom V).
+
+Definition type_qualifier : Type := type_qualifier_of (V := value).
+
+Definition tqual {V : Type} `{ValueSig V}
+    (B : gset nat) (d : aset)
+    (prop : gmap nat V → gmap atom V → gmap atom V → Prop) :
+    type_qualifier_of (V := V) :=
+  qual B d prop.
 
 (** ** Locally-nameless infrastructure *)
 
-Definition qual_open (k : nat) (s : value) (q : type_qualifier) : type_qualifier :=
-  match q with
-  | qual vals prop => qual (vmap (open_value k s) vals) prop
-  end.
+Definition qual_open {V : Type} `{ValueSig V}
+    (k : nat) (x : atom) (q : type_qualifier_of (V := V)) : type_qualifier_of (V := V) :=
+  qual_open_atom k x q.
 
-Definition qual_fv (q : type_qualifier) : aset :=
-  match q with
-  | qual vals _ => Vector.fold_right (fun v s => fv_value v ∪ s) vals ∅
-  end.
+Definition qual_open_with_value (k : nat) (v : value) (q : type_qualifier) :
+    type_qualifier :=
+  qual_open_value k v q.
+
+Definition qual_fv {V : Type} `{ValueSig V} (q : type_qualifier_of (V := V)) : aset :=
+  qual_dom q.
 
 Definition qual_subst_one (x : atom) (v : value) (q : type_qualifier) : type_qualifier :=
-  match q with
-  | qual vals prop => qual (vmap (value_subst x v) vals) prop
-  end.
+  qual_subst_value x v q.
 
-Definition qual_subst (σ : Store) (q : type_qualifier) : type_qualifier :=
-  match q with
-  | qual vals prop => qual (vmap (value_subst_all σ) vals) prop
-  end.
+Definition qual_subst (σ : gmap atom value) (q : type_qualifier) : type_qualifier :=
+  qual_subst_map σ q.
 
-#[global] Instance open_qual_inst      : Open value type_qualifier := qual_open.
+#[global] Instance open_qual_inst      : Open value type_qualifier := qual_open_with_value.
+#[global] Instance open_qual_atom_inst : Open atom type_qualifier := qual_open.
 #[global] Instance stale_qual_inst     : Stale type_qualifier := qual_fv.
 #[global] Instance subst_qual_inst     : SubstV value type_qualifier := qual_subst_one.
-#[global] Instance substM_qual_inst    : SubstM Store type_qualifier := qual_subst.
+#[global] Instance substM_qual_inst    : SubstM (gmap atom value) type_qualifier := qual_subst.
 Arguments open_qual_inst /.
+Arguments open_qual_atom_inst /.
 Arguments stale_qual_inst /.
 Arguments subst_qual_inst /.
 Arguments substM_qual_inst /.
 
-Notation "q '^q^' x" := (qual_open 0 (vfvar x) q) (at level 20).
+Notation "q '^q^' x" := (qual_open 0 x q) (at level 20).
 Notation "'{' x ':=' v '}q' q" := (qual_subst_one x v q)
   (at level 20, x constr, v constr, format "{ x := v }q  q").
 
 (** ** Local closure *)
 
-Inductive lc_qualifier : type_qualifier → Prop :=
-  | LCQ_qual n vals prop :
-      Vector.Forall lc_value vals →
-      lc_qualifier (@qual n vals prop).
+Definition lc_qualifier (q : type_qualifier) : Prop :=
+  qual_bvars q = ∅.
 
 #[global] Instance lc_qual_inst : Lc type_qualifier := lc_qualifier.
 Arguments lc_qual_inst /.
-#[global] Hint Constructors lc_qualifier : core.
 
 (** ** Conjunction of two shallow qualifiers *)
 
 Definition qualifier_and (q1 q2 : type_qualifier) : type_qualifier :=
   match q1, q2 with
-  | qual vals1 prop1, qual vals2 prop2 =>
-      qual (vals1 +++ vals2) (fun v =>
-        let '(v1, v2) := Vector.splitat _ v in prop1 v1 ∧ prop2 v2)
+  | qual B1 d1 prop1, qual B2 d2 prop2 =>
+      qual (B1 ∪ B2) (d1 ∪ d2) (fun β σ ρ => prop1 β σ ρ ∧ prop2 β σ ρ)
   end.
 
 Notation "q1 '&q' q2" := (qualifier_and q1 q2) (at level 40).
 
 (** ** Denotation helpers *)
 
-Fixpoint eval_vals (σ : Store) {n} (vals : vec value n) : option (vec constant n) :=
-  match vals with
-  | [#]       => Some [#]
-  | v ::: vs  =>
-      match value_subst_all σ v with
-      | vconst c =>
-          match eval_vals σ vs with
-          | Some cs => Some (c ::: cs)
-          | None    => None
-          end
-      | _ => None
-      end
-  end.
-
-Definition qual_interp (σ : Store) (q : type_qualifier) : Prop :=
+Definition qual_interp_full
+    (β : gmap nat value) (σ ρ : gmap atom value) (q : type_qualifier) : Prop :=
   match q with
-  | qual vals prop =>
-      match eval_vals σ vals with
-      | Some cs => prop cs
-      | None    => False
-      end
+  | qual B d prop =>
+      prop (map_restrict value β B) (store_restrict σ d) (store_restrict ρ d)
   end.
 
-Definition qual_interp_cl (q : type_qualifier) (σ : Store) : Prop :=
+Definition qual_interp (σ : gmap atom value) (q : type_qualifier) : Prop :=
+  qual_interp_full ∅ σ σ q.
+
+Definition qual_interp_cl (q : type_qualifier) (σ : gmap atom value) : Prop :=
   qual_interp σ q.
 
-#[global] Instance denot_qual_inst : Denotation type_qualifier (Store → Prop) :=
+#[global] Instance denot_qual_inst : Denotation type_qualifier (gmap atom value → Prop) :=
   qual_interp_cl.
 Arguments denot_qual_inst /.
 
@@ -109,8 +96,34 @@ Parameter type_qualifier_to_logic : type_qualifier → logic_qualifier.
 
 (** ** Standard notations from UnderType *)
 
+Fixpoint bv_value (v : value) : gset nat :=
+  match v with
+  | vconst _ => ∅
+  | vfvar _ => ∅
+  | vbvar k => {[k]}
+  | vlam _ e => bv_tm e
+  | vfix _ vf => bv_value vf
+  end
+with bv_tm (e : tm) : gset nat :=
+  match e with
+  | tret v => bv_value v
+  | tlete e1 e2 => bv_tm e1 ∪ bv_tm e2
+  | tprim _ v => bv_value v
+  | tapp v1 v2 => bv_value v1 ∪ bv_value v2
+  | tmatch v et ef => bv_value v ∪ bv_tm et ∪ bv_tm ef
+  end.
+
+Definition denote_value (β : gmap nat value) (σ : gmap atom value) (v : value) : option value :=
+  match v with
+  | vbvar k => β !! k
+  | vfvar x => σ !! x
+  | vconst c => Some (vconst c)
+  | _ => Some v
+  end.
+
 Definition mk_q_eq (v1 v2 : value) : type_qualifier :=
-  qual [# v1; v2] (fun v => v !!! 0%fin = v !!! 1%fin).
+  qual (bv_value v1 ∪ bv_value v2) (fv_value v1 ∪ fv_value v2)
+    (fun β σ _ => denote_value β σ v1 = denote_value β σ v2).
 
 Notation "'b0:v=' v" := (mk_q_eq (vbvar 0) v)
   (at level 5, format "b0:v= v").
@@ -119,8 +132,8 @@ Notation "'b0:x=' x" := (mk_q_eq (vbvar 0) (vfvar x))
 Notation "'b0:c=' c" := (mk_q_eq (vbvar 0) (vconst c))
   (at level 5, format "b0:c= c").
 
-Definition qual_top : type_qualifier := qual [#] (fun _ => True).
-Definition qual_bot : type_qualifier := qual [#] (fun _ => False).
+Definition qual_top : type_qualifier := qual ∅ ∅ (fun _ _ _ => True).
+Definition qual_bot : type_qualifier := qual ∅ ∅ (fun _ _ _ => False).
 Notation "⊤q" := qual_top.
 Notation "⊥q" := qual_bot.
 
@@ -138,7 +151,7 @@ Lemma qual_subst_intro x v (q : type_qualifier) :
   x # q → lc_value v → {x := v}q (q ^q^ x) = {0 ~> v} q.
 Proof. Admitted.
 
-Lemma qual_interp_subst_compose (σ_X σ : Store) (q : type_qualifier) :
+Lemma qual_interp_subst_compose (σ_X σ : gmap atom value) (q : type_qualifier) :
   store_compat σ_X σ →
   qual_interp σ (qual_subst σ_X q) ↔ qual_interp (σ_X ∪ σ) q.
 Proof. Admitted.
