ChoicePrelude/Qualifier.v
@@ -1,0 +1,67 @@
+(** * Generic shallow qualifiers *)
+
+From ChoicePrelude Require Export Prelude Store.
+
+Section Qualifier.
+
+Context {V A : Type} `{ValueSig V}.
+
+Local Notation BStoreT := (gmap nat V) (only parsing).
+Local Notation StoreT := (gmap atom V) (only parsing).
+
+Inductive qualifier : Type :=
+  | qual (B : gset nat) (d : aset) (prop : BStoreT → StoreT → A → Prop).
+
+Definition qual_bvars (q : qualifier) : gset nat :=
+  match q with
+  | qual B _ _ => B
+  end.
+
+Definition qual_dom (q : qualifier) : aset :=
+  match q with
+  | qual _ d _ => d
+  end.
+
+Definition qual_prop (q : qualifier) : BStoreT → StoreT → A → Prop :=
+  match q with
+  | qual _ _ p => p
+  end.
+
+Definition qual_open_value (k : nat) (v : V) (q : qualifier) : qualifier :=
+  match q with
+  | qual B d p =>
+      if decide (k ∈ B) then
+        qual (B ∖ {[k]}) d (λ β σ a, p (<[k := v]> β) σ a)
+      else q
+  end.
+
+Definition qual_open_atom (k : nat) (x : atom) (q : qualifier) : qualifier :=
+  match q with
+  | qual B d p =>
+      if decide (k ∈ B) then
+        qual (B ∖ {[k]}) ({[x]} ∪ d)
+          (λ β σ a, ∃ v, σ !! x = Some v ∧ p (<[k := v]> β) σ a)
+      else q
+  end.
+
+Definition qual_subst_value (x : atom) (v : V) (q : qualifier) : qualifier :=
+  match q with
+  | qual B d p =>
+      if decide (x ∈ d) then
+        qual B (d ∖ {[x]}) (λ β σ a, p β (<[x := v]> σ) a)
+      else q
+  end.
+
+Definition qual_subst_map (θ : StoreT) (q : qualifier) : qualifier :=
+  match q with
+  | qual B d p =>
+      qual B (d ∖ dom θ) (λ β σ a, p β (θ ∪ σ) a)
+  end.
+
+Definition lc_qualifier (q : qualifier) : Prop :=
+  qual_bvars q = ∅.
+
+#[global] Instance stale_qualifier : Stale qualifier := qual_dom.
+Arguments stale_qualifier /.
+
+End Qualifier.
