ChoicePrelude/Store.v
@@ -1,0 +1,226 @@
+(** * Stores and polymorphic finite-map restriction *)
+
+From ChoicePrelude Require Export Prelude MapFilterDom.
+
+(** ** Polymorphic finite-map compatibility and restriction *)
+
+Section MapOps.
+
+Context `{Countable K}.
+Context {A : Type}.
+
+Definition map_compat (m1 m2 : gmap K A) : Prop :=
+  ∀ x v1 v2, m1 !! x = Some v1 → m2 !! x = Some v2 → v1 = v2.
+
+Definition map_restrict (m : gmap K A) (X : gset K) : gmap K A :=
+  filter (λ '(k, _), k ∈ X) m.
+
+Lemma map_compat_refl m : map_compat m m.
+Proof.
+  unfold map_compat. intros x v1 v2 H1 H2. hauto.
+Qed.
+
+Lemma map_compat_sym m1 m2 :
+  map_compat m1 m2 → map_compat m2 m1.
+Proof. unfold map_compat. intros Hc x v1 v2 H1 H2. hauto. Qed.
+
+Lemma map_compat_union m1 m2 :
+  map_compat m1 m2 →
+  map_compat (m1 ∪ m2) (m1 ∪ m2).
+Proof. unfold map_compat. intros Hc x v1 v2 H1 H2. hauto. Qed.
+
+Lemma map_restrict_dom m X :
+  dom (map_restrict m X) = dom m ∩ X.
+Proof.
+  unfold map_restrict. apply dom_gmap_filter_key_in_pair.
+Qed.
+
+Lemma map_restrict_idemp m X :
+  dom m ⊆ X → map_restrict m X = m.
+Proof.
+  unfold map_restrict. intros Hsub. apply map_filter_id.
+  intros i x Hx. apply elem_of_dom_2 in Hx. set_solver.
+Qed.
+
+Lemma map_restrict_restrict m X Y :
+  map_restrict (map_restrict m X) Y = map_restrict m (X ∩ Y).
+Proof.
+  unfold map_restrict.
+  setoid_rewrite map_filter_filter.
+  apply map_filter_ext.
+  intros i x Hx. apply elem_of_dom_2 in Hx. set_solver.
+Qed.
+
+Lemma map_restrict_lookup_some m X x y :
+  map_restrict m X !! x = Some y → x ∈ X ∧ m !! x = Some y.
+Proof.
+  unfold map_restrict. intro Hlookup.
+  apply map_lookup_filter_Some in Hlookup.
+  destruct Hlookup as [H1 H2]. split; [exact H2 | exact H1].
+Qed.
+
+End MapOps.
+
+Arguments map_compat {_ _ _} _ _ /.
+Arguments map_restrict {_ _ _} _ _ /.
+
+(** ** Atom-keyed stores *)
+
+Section Store.
+
+Context {V : Type} `{ValueSig V}.
+
+Definition Store : Type := gmap atom V.
+
+Definition store_compat (s1 s2 : Store) : Prop := map_compat V s1 s2.
+
+Definition store_restrict (s : Store) (X : aset) : Store := map_restrict V s X.
+
+Lemma store_compat_refl s : store_compat s s.
+Proof.
+  unfold store_compat. intros x v1 v2 H1 H2. hauto.
+Qed.
+
+Lemma store_compat_sym s1 s2 :
+  store_compat s1 s2 → store_compat s2 s1.
+Proof. unfold store_compat. intros Hc x v1 v2 H1 H2. hauto. Qed.
+
+Lemma store_compat_union s1 s2 :
+  store_compat s1 s2 →
+  store_compat (s1 ∪ s2) (s1 ∪ s2).
+Proof. unfold store_compat. intros Hc x v1 v2 H1 H2. hauto. Qed.
+
+Lemma store_restrict_dom s X :
+  dom (store_restrict s X) = dom s ∩ X.
+Proof.
+  unfold store_restrict. apply dom_gmap_filter_key_in_pair.
+Qed.
+
+Lemma store_restrict_idemp s X :
+  dom s ⊆ X → store_restrict s X = s.
+Proof.
+  unfold store_restrict. intros Hsub. apply map_filter_id.
+  intros i x Hx. apply elem_of_dom_2 in Hx. set_solver.
+Qed.
+
+Lemma store_restrict_restrict s X Y :
+  store_restrict (store_restrict s X) Y = store_restrict s (X ∩ Y).
+Proof.
+  unfold store_restrict, map_restrict.
+  setoid_rewrite map_filter_filter.
+  apply map_filter_ext.
+  intros i x Hx. apply elem_of_dom_2 in Hx. set_solver.
+Qed.
+
+Lemma store_union_dom s1 s2 :
+  store_compat s1 s2 →
+  dom (s1 ∪ s2) = dom s1 ∪ dom s2.
+Proof.
+  intros Hcomp. setoid_rewrite dom_union_L. auto.
+Qed.
+
+Lemma store_restrict_induce_disjoint s1 s2 :
+  s1 ##ₘ (store_restrict s2 (dom s2 ∖ dom s1)) ∧
+  s1 ∪ s2 = s1 ∪ (store_restrict s2 (dom s2 ∖ dom s1)).
+Proof.
+  pose (s2' := store_restrict s2 (dom s2 ∖ dom s1)).
+  split.
+  - rewrite map_disjoint_alt. intros i.
+    destruct (decide (i ∈ dom s1)).
+    + right.
+      apply map_lookup_filter_None_2. right.
+      intros x Hx Hi%elem_of_difference.
+      destruct Hi as [_ Hi']. by apply Hi'.
+    + left. by apply not_elem_of_dom.
+  - apply map_eq. intros i.
+    destruct (s1 !! i) as [x|] eqn:E1.
+    + rewrite (lookup_union_l' s1 s2 i) by (by exists x; exact E1).
+      rewrite (lookup_union_l' s1 s2' i) by (by exists x; exact E1).
+      reflexivity.
+    + rewrite (lookup_union_r s1 s2 i) by done.
+      rewrite (lookup_union_r s1 s2' i) by done.
+      destruct (s2 !! i) as [y|] eqn:E2.
+      * etrans.
+        -- exact E2.
+        -- symmetry. unfold s2', store_restrict.
+           apply map_lookup_filter_Some_2; first exact E2.
+           apply elem_of_difference. split.
+           ++ by apply elem_of_dom; exists y.
+           ++ by apply not_elem_of_dom.
+      * apply eq_trans with (@None V); first exact E2.
+        symmetry. unfold s2', store_restrict.
+        apply map_lookup_filter_None. left. exact E2.
+Qed.
+
+Lemma store_restrict_union s1 s2 X :
+  store_compat s1 s2 →
+  store_restrict (s1 ∪ s2) X = store_restrict s1 X ∪ store_restrict s2 X.
+Proof.
+  intros Hcomp.
+  unfold store_restrict, map_restrict.
+  setoid_rewrite gmap_filter_key_pair.
+  apply map_eq. intros i.
+  rewrite option_eq. intros x.
+  setoid_rewrite map_lookup_filter_Some.
+  setoid_rewrite lookup_union_Some_raw.
+  setoid_rewrite map_lookup_filter_Some.
+  setoid_rewrite map_lookup_filter_None.
+  simpl. split.
+  - intros [[H1|[H1 H2]] HP].
+    + left. eauto.
+    + right. split. { left. exact H1. } eauto.
+  - intros [[H1 HP]|[[H1|H1] [H2 HP]]].
+    + split. { left. exact H1. } exact HP.
+    + split. { right. eauto. } exact HP.
+    + destruct (s1 !! i) as [y|] eqn:Ey.
+      * exfalso. exact (H1 y Ey HP).
+      * split. { right. eauto. } exact HP.
+Qed.
+
+Lemma store_restrict_lookup_some s X x y :
+  store_restrict s X !! x = Some y → x ∈ X ∧ s !! x = Some y.
+Proof.
+  unfold store_restrict. intro Hlookup.
+  apply map_lookup_filter_Some in Hlookup.
+  destruct Hlookup as [H1 H2]. split; [exact H2 | exact H1].
+Qed.
+
+Lemma store_compat_restrict s1 s2 X :
+  store_compat s1 s2 → store_compat (store_restrict s1 X) (store_restrict s2 X).
+Proof.
+  unfold store_compat. intros Hcomp x y z H2 H3.
+  apply store_restrict_lookup_some in H2.
+  apply store_restrict_lookup_some in H3.
+  hauto.
+Qed.
+
+Lemma store_compat_restrict_eq s1 s2 :
+  store_compat s1 s2 →
+  dom s1 ⊆ dom s2 →
+  store_restrict s2 (dom s1) = s1.
+Proof.
+  unfold store_compat. intros Hcomp Hsub.
+  apply map_eq. intros i.
+  destruct (s1 !! i) as [v1|] eqn:H1.
+  - assert (i ∈ dom s2) as Hin2 by (apply Hsub; apply elem_of_dom; eauto).
+    pose (H2 := lookup_lookup_total_dom s2 i Hin2).
+    assert (H2' : s2 !! i = Some v1).
+    { transitivity (Some (s2 !!! i)); first exact H2.
+      f_equal. symmetry. exact (Hcomp i v1 (s2 !!! i) H1 H2). }
+    etrans.
+    + unfold store_restrict, map_restrict.
+      apply map_lookup_filter_Some_2; last by apply elem_of_dom; eauto.
+      exact H2'.
+    + symmetry. exact H1.
+  - unfold store_restrict, map_restrict.
+    etrans.
+    + apply map_lookup_filter_None. right.
+      intros v2 H2 Hin.
+      apply not_elem_of_dom in H1. set_solver.
+    + symmetry. exact H1.
+Qed.
+
+End Store.
+
+#[global] Instance stale_store {A} : Stale (gmap atom A) := dom.
+Arguments stale_store /.
